Cleaning: SSReflect idioms, move some lemmas, renaming

yalla/mll_pn_to_seq.v
@@ -41,11 +41,7 @@ Lemma bridge_sym : local_symmetric bridge.
 Proof. move=> v e1 e2 _ _. rewrite /bridge. lia. Qed.
 
 Lemma bridge_trans : local_transitive bridge.
-Proof.
-  move=> v e1 e2 e3 _ _ _.
-  rewrite /bridge.
-  by move=> /andP[/andP[-> _] _] /andP[/andP[_ ->] ->].
-Qed.
+Proof. move=> v e1 e2 e3 _ _ _. rewrite /bridge. lia. Qed.
 
 Definition T : finType :=
   { x : G * (option (edge G)) | (vlabel x.1 != c) &&
@@ -59,19 +55,19 @@ Definition v_of_t (u : T) : G :=
 Definition e_of_t (u : T) : option (edge G * bool) :=
   match u with
   | exist (_, Some e) _ => Some (forward e)
-  | exist (_, None) _ => None
+  | exist (_, None)   _ => None
   end.
 
-Definition vertex_finPOrderType3 : finPOrderType tt :=
-  vertex_finPOrderType2 bridge v_of_t e_of_t.
+Definition seq_finPOrderType : finPOrderType tt :=
+  T_finPOrderType_bridge bridge v_of_t e_of_t.
 
 Lemma t_of_b_helper (e : edge G * bool) (e' : edge G) :
-  bridge (utarget e) e.1 e' -> e.1 <> e' ->
+  bridge (utarget e) e.1 e' ->
   (vlabel (target e.1) != c) && (target e.1 == target e.1).
-Proof. by move => /andP[/andP[/eqP--> _] /eqP-->] /=. Qed.
+Proof. by move=> /andP[/andP[/eqP--> _] /eqP-->] /=. Qed.
 
 Definition t_of_b (e : edge G * bool) e' (B : bridge (utarget e) e.1 e') (N : e.1 <> e') : T :=
-  Sub (target e.1, Some e.1) (t_of_b_helper B N).
+  Sub (target e.1, Some e.1) (t_of_b_helper B).
 
 Lemma eq_switching_is_bridge (e f : edge G) :
   switching e = switching f -> e <> f -> bridge (target e) e f.
@@ -89,6 +85,7 @@ Qed.
 Lemma correct_is_correct :
   uacyclic (@switching _ G) -> correct bridge.
 Proof.
+(* By contradiction, a simple path p has no bridge but its edges are not unique by switching. *)
   move=> U.
   rewrite /correct. apply/forallP. move=> [p P] /=.
   apply/implyP => bridge_free_p.
@@ -106,15 +103,14 @@ Proof.
   apply/(uniqP (switching e.1)) => i j.
   rewrite size_map !inE => i_lt j_lt.
   rewrite !(nth_map e) // => bridge_nth.
-  case/boolP: (i == j) => /eqP-i_neq_j //.
-  exfalso.
+  case/boolP: (i == j) => /eqP-i_neq_j //. exfalso.
+(* The equality on switching yields a bridge. *)
   apply eq_switching_is_bridge in bridge_nth; last first.
   { move=> F.
     apply uniq_fst_simple_upath in P.
     move: P => /uniqP => /(_ e.1)/(_ i j).
-    rewrite size_map => P.
-    contradict i_neq_j. apply P; clear P; try by [].
-    by rewrite !(nth_map e). }
+    rewrite size_map !(nth_map e) // => P.
+    contradict i_neq_j. by apply P. }
   move: bridge_nth. rewrite /bridge eq_refl /= eq_sym => /andP[/eqP-target_i_j parr_i_j].
   wlog {i_neq_j} i_lt_j : i j i_lt j_lt target_i_j parr_i_j / i < j.
   { clear P bridge_free_p no_bridge => Wlog.
@@ -127,31 +123,17 @@ Proof.
    thus they are consecutive (modulo p), contradicting bridge_freeness. *)
   have /orP[/andP[/andP[/eqP-? i2] j2] | /andP[/andP[/andP[/eqP-? /eqP-?] i2] j2]] :=
     @same_target_are_consecutive _ _ _ (e :: p) e i j P i_lt j_lt i_lt_j target_i_j.
-  - subst j. clear i_lt i_lt_j.
+  - subst j. clear i_lt i_lt_j P no_bridge.
     contradict bridge_free_p. apply/negP.
-    assert (ep_eq : e :: p = take i (e :: p) ++
-      [:: nth e (e :: p) i; nth e (e :: p) (i + 1)] ++ drop (i + 2) (e :: p)).
-    { clear - j_lt.
-      move: i j_lt.
-      set p' := e :: p. clearbody p'. clear p.
-      induction p' as [ | e' p IH] => i //= j_lt.
-      destruct i as [ | i].
-      + rewrite /= nth0 drop1. by destruct p.
-      + by rewrite {1}(IH i). } (* TODO lemma for this *)
-    rewrite ep_eq !nb_bridges_cat /=.
+    rewrite (take_nth_drop2 e j_lt) nb_bridges_cat /=.
     enough (bridge (utarget (nth e (e :: p) i)) (nth e (e :: p) i).1
       (nth e (e :: p) (i + 1)).1) as -> by lia.
-    move: i2 j2.
-    destruct (nth e (e :: p) i) as [ei []], (nth e (e :: p) (i + 1)) as [ej []]
-      => //= _ _.
+    destruct (nth e (e :: p) i) as [ei []], (nth e (e :: p) (i + 1)) as [ej []] => //=.
     by rewrite /bridge parr_i_j target_i_j eq_refl.
-  - subst i j.
+  - subst i j. clear i_lt j_lt P bridge_free_p.
     rewrite nth_last in target_i_j, j2. simpl in *.
-    destruct p as [ | ep p]; first by []. simpl in *.
-    assert (no_bridge' : ~~ bridge (utarget e) e.1 ep.1).
-    { clear - bridge_free_p. lia. }
-    clear bridge_free_p.
-    destruct e as [e []]; first by []; simpl in *.
+    destruct e as [e []]; first by []. clear i2. simpl in *.
+    destruct p as [ | ep p]; first by []. clear i_lt_j. simpl in *.
     contradict no_bridge. apply/negP/negPn.
     by rewrite /bridge -target_i_j parr_i_j !eq_refl.
 Qed.
@@ -163,32 +145,32 @@ Section Sequentializable.
 Context {G : proof_net}.
 
 Notation bridge := (@bridge G).
-Notation vertex_finPOrderType3 := (@vertex_finPOrderType3 G).
+Notation seq_finPOrderType := (@seq_finPOrderType G).
 
 Fact is_correct_bridge : correct bridge.
 Proof. apply correct_is_correct. by destruct (p_correct G). Qed.
 
 (* A vertex v which is maximal is terminal.
    Or by contrapose, a non-terminal element cannot be maximal. *)
-Lemma no_terminal_is_no_max (v : vertex_finPOrderType3) :
-  ~~ terminal (v_of_t v) -> exists U, (v : vertex_finPOrderType3) < U.
+Lemma no_terminal_is_no_max (v : seq_finPOrderType) :
+  ~~ terminal (v_of_t v) -> exists U, v < U.
 Proof.
   move=> not_terminal_v.
   destruct v as [[v f] V]. simpl in *.
   apply not_terminal in not_terminal_v as [e [se_is_v te_not_c]]; last first.
-  { clear not_terminal_v. by move: V => /= /andP[/eqP-? _]. }
+  { by move: V => /= /andP[/eqP-? _]. }
   assert (H : (vlabel (target e) != c) && (target e == target e)).
-  { rewrite eq_refl andb_true_r. by apply /eqP. }
+  { rewrite eq_refl andb_true_r. by apply/eqP. }
   exists (exist _ (target e, Some e) H).
-  apply /existsP. exists (Sub [:: forward e] (simple_upath_edge _)).
+  apply/existsP. exists (Sub [:: forward e] (simple_upath_edge _)).
   rewrite /pre_ordering /Psource /Ptarget /= se_is_v /= !eq_refl !andb_true_r /= {H}.
   move: V => /andP[/eqP-v_not_c vf].
   assert (te_neq_v : v <> target e).
   { move=> v_eq.
     contradict se_is_v. rewrite v_eq.
     apply no_selfloop. }
-  repeat (apply /andP; split).
-  - by apply /eqP.
+  repeat (apply/andP; split).
+  - by apply/eqP.
   - destruct f as [f | ]; last by [].
     rewrite /= /bridge (eqP vf) eq_refl /= negb_andb.
     apply/andP. split.
@@ -206,10 +188,10 @@ Proof.
     wlog {v_in_targets_p} v_eq_target_p : p P Pnc sp_eq_te fst_p_not_e
       bridge_free_p no_bridge_p_e / (v = upath_target (target e) p).
     { move {te_not_c v_not_c vf} => Wlog.
-      revert v_in_targets_p => /mapP[a a_in_p v_eq_ta].
-      assert (H : (fun b => v == utarget b) a) by by apply /eqP.
+      move: v_in_targets_p => /mapP[a a_in_p v_eq_ta].
+      assert (H : (fun b => v == utarget b) a) by by apply/eqP.
       destruct (in_elt_sub_fst H a_in_p) as [[n N] [a' [p_eq [v_eq_ta' a'_fst]]]].
-      revert v_eq_ta' => {H} /eqP-v_eq_ta'.
+      move: v_eq_ta' => {H} /eqP-v_eq_ta'.
       rewrite -cat_rcons in p_eq.
       apply (Wlog (rcons (take (Ordinal N) p) a')); clear Wlog.
       - rewrite p_eq in P. by apply simple_upath_prefix in P.
@@ -218,30 +200,30 @@ Proof.
         destruct n as [ | n].
         + simpl in *. inversion p_eq. subst ep.
           destruct a' as [a' []]; [ | apply nesym]; apply no_selfloop.
-        + move => /= Ta'.
+        + move=> /= Ta'.
           simpl in sp_eq_te.
           contradict te_neq_v. by rewrite v_eq_ta' -Ta' sp_eq_te.
-      - revert sp_eq_te. by rewrite {1}p_eq map_cat !map_rcons head_cat !head_rcons.
-      - revert fst_p_not_e. by rewrite {1}p_eq head_cat !head_rcons.
-      - revert bridge_free_p. rewrite {1}p_eq nb_bridges_cat. clear. simpl. lia.
-      - revert no_bridge_p_e. by rewrite {1}p_eq head_cat !head_rcons.
+      - move: sp_eq_te. by rewrite {1}p_eq map_cat !map_rcons head_cat !head_rcons.
+      - move: fst_p_not_e. by rewrite {1}p_eq head_cat !head_rcons.
+      - move: bridge_free_p. rewrite {1}p_eq nb_bridges_cat. clear. simpl. lia.
+      - move: no_bridge_p_e. by rewrite {1}p_eq head_cat !head_rcons.
       - by rewrite /= map_rcons last_rcons v_eq_ta'. }
 (* The path e :: p contradicts correctness. *)
     assert (EP : simple_upath (forward e :: p)).
     { rewrite simple_upath_cons P /= se_is_v -{1}sp_eq_te.
       destruct p as [ | ep p]; first by [].
-      revert fst_p_not_e Pnc => /= /eqP-fst_p_not_e /eqP-Pnc.
-      rewrite /= eq_refl eq_sym fst_p_not_e Pnc /= andb_true_r v_eq_target_p.
-      rewrite /= in_cons negb_orb eq_sym Pnc /=.
-      revert P. rewrite /simple_upath /= eq_refl /= in_cons negb_orb.
-      move => /andP[/andP[/andP[_ /orP[/andP[_ -> //] | F]] _] _].
-      by rewrite eq_sym F in Pnc. }
+      move: fst_p_not_e Pnc => /= /eqP-fst_p_not_e /eqP-Pnc.
+      rewrite eq_refl eq_sym fst_p_not_e Pnc andb_true_r v_eq_target_p
+        in_cons negb_orb eq_sym Pnc /=.
+      move: P. rewrite /simple_upath /= eq_refl /= in_cons negb_orb.
+      rewrite eq_sym in Pnc. rewrite (negPf Pnc) orb_false_r /=.
+      by move=> /andP[/andP[/andP[_ ->] _] _]. }
     have /forallP/(_ (Sub _ EP)) /= H := is_correct_bridge.
     contradict H. apply/negP.
-    rewrite !negb_imply se_is_v v_eq_target_p /= eq_refl /=.
+    rewrite !negb_imply se_is_v v_eq_target_p eq_refl /=.
     apply/andP. split.
     + rewrite /= bridge_free_p.
-      destruct p as [ | ep p]; first by []. simpl.
+      destruct p as [ | ep p]; first by [].
       by rewrite (negPf no_bridge_p_e).
     + rewrite /bridge !negb_andb.
       apply/orP. left. apply/orP. left.
@@ -253,21 +235,20 @@ Theorem exists_terminal_splitting :
   { v : G | splitting bridge v && terminal v }.
 Proof.
   apply/sigW.
-  assert (u : vertex_finPOrderType3).
+  assert (u : seq_finPOrderType).
   { destruct (has_ax G) as [u U].
     exists (u, None). by rewrite U. }
   induction u as [u IH] using (well_founded_ind gt_wf).
   case/boolP: (splitting bridge (v_of_t u) && terminal (v_of_t u)) => split_u.
   { by exists (v_of_t u). }
-  enough (exists v, (u : vertex_finPOrderType3) < v) as [v ?]
+  enough (exists v, (u : seq_finPOrderType) < v) as [v ?]
     by by apply (IH v).
   move: split_u => /nandP[split_u | term_u]; [ | exact (no_terminal_is_no_max term_u)].
   refine (@no_splitting_is_no_max _ _ _ _ bridge_sym bridge_trans _ v_of_t e_of_t
     _ t_of_b _ _ is_correct_bridge split_u).
-  - move=> [e []] e' //=.
-    rewrite /bridge => /andP[/andP[/eqP-F _] _].
+  - move=> [e []] e' //= /andP[/andP[/eqP-F _] _].
     contradict F. apply nesym, no_selfloop.
-  - by elim => [[? [? | ]] //= /andP[_ ->]].
+  - by move=> [[? [? | ]] //= /andP[_ ->]].
 Qed.
 
 End Sequentializable.
