yalla/mll_pn_to_seq_parr.v
@@ -1,4 +1,4 @@
-(* Sequentialisation - A terminal parr vertex is sequentializing *)
+(* Sequentialisation - A terminal ⅋ is sequentializing *)
 
 From Coq Require Import Bool.
 From OLlibs Require Import dectype.
@@ -7,7 +7,7 @@ From mathcomp Require Import all_ssreflect.
 Set Warnings "notation-overridden".
 From GraphTheory Require Import preliminaries mgraph setoid_bigop structures bij.
 
-From Yalla Require Export mll_prelim graph_more upath supath mll_def mll_basic mll_seq_to_pn
+From Yalla Require Export mll_prelim graph_more upath mll_def mll_basic mll_seq_to_pn
   mll_pn_to_seq_def.
 
 Import EqNotations.
@@ -31,13 +31,10 @@ Notation base_graph := (graph (flat rule) (flat (formula * bool))).
 Notation graph_data := (@graph_data atom).
 Notation proof_structure := (@proof_structure atom).
 Notation proof_net := (@proof_net atom).
-Notation switching := (@switching atom).
-Notation switching_left := (@switching_left atom).
 
 
 Section Rem_node.
-Context {G : proof_structure} {v : G}.
-Hypothesis (V : vlabel v = ⊗ \/ vlabel v = ⅋) (T : terminal v).
+Context {G : proof_structure} {v : G} (V : vlabel v = ⊗ \/ vlabel v = ⅋) (T : terminal v).
 
 (* Vertices neighbourhing v *)
 Local Notation elv := (left V).
@@ -47,13 +44,13 @@ Local Notation lv := (source elv).
 Local Notation rv := (source erv).
 Local Notation cv := (target ecv).
 
-(** Base graph for removing a node and its eventual conclusion *) (* TODO faire comme add_node des cas selon vlabel_v pour factoriser ? *)
+(** Base graph for removing a node and its conclusion *)
 Definition rem_node_graph_1 := induced ([set: G] :\ v :\ cv).
 
 (* Then add new conclusions *)
 Lemma lv_inside : lv \in setT :\ v :\ cv.
 Proof.
-  rewrite !in_set !in_set1. splitb; apply /eqP => F.
+  rewrite !in_set !in_set1 andb_true_r. splitb; apply/eqP => F.
   - assert (P : walk lv lv [:: elv ; ecv]) by by rewrite /= F ccl_e left_e; splitb.
     by specialize (ps_acyclic P).
   - assert (FF : lv = target elv) by by rewrite left_e.
@@ -62,7 +59,7 @@ Qed.
 
 Lemma rv_inside : rv \in setT :\ v :\ cv.
 Proof.
-  rewrite !in_set !in_set1. splitb; apply /eqP => F.
+  rewrite !in_set !in_set1 andb_true_r. splitb; apply/eqP => F.
   - assert (P : walk rv rv [:: erv ; ecv]) by by rewrite /= F ccl_e right_e; splitb.
     by specialize (ps_acyclic P).
   - assert (FF : rv = target erv) by by rewrite right_e.
@@ -74,10 +71,10 @@ Definition rem_node_graph :=
                      (inl (Sub lv lv_inside)) c (flabel elv).
 
 Lemma vlabel_cv : vlabel cv = c.
-Proof. apply /eqP. by rewrite -terminal_tens_parr. Qed.
+Proof. apply/eqP. by rewrite -terminal_tens_parr. Qed.
 
 Lemma v_neq_cv : v <> cv.
-Proof. intro F. have := vlabel_cv. rewrite -F. by destruct V as [V' | V']; rewrite V'. Qed.
+Proof. move=> F. have := vlabel_cv. rewrite -F. by destruct V as [V' | V']; rewrite V'. Qed.
 
 (* Give its order *)
 Definition rem_node_transport (e : edge G) : edge rem_node_graph :=
@@ -94,18 +91,17 @@ Definition rem_node_graph_data := {|
 
 Lemma rem_node_removed : edge_set (setT :\ v :\ cv) = setT :\ elv :\ erv :\ ecv.
 Proof.
-  assert (C := vlabel_cv).
-  apply /setP => a. rewrite !in_set !in_set1 !andb_true_r.
+  apply/setP => a. rewrite !in_set !in_set1 !andb_true_r.
   destruct (eq_comparable a ecv) as [? | Hc];
   [ | destruct (eq_comparable a erv) as [? | Hr]];
   [ | | destruct (eq_comparable a elv)];
   try by (subst a; rewrite ?left_e ?right_e !eq_refl ?andb_false_r).
-  assert (a != ecv /\ a != erv /\ a != elv) as [-> [-> ->]] by by splitb; apply /eqP.
-  simpl. splitb; apply /eqP.
-  - by apply no_source_c.
-  - intros ?. contradict Hc. by apply ccl_eq.
-  - intros ?. contradict Hc. by apply one_target_c.
-  - intros ?. contradict Hr. by apply right_eq2.
+  assert (a != ecv /\ a != erv /\ a != elv) as [-> [-> ->]] by by splitb; apply/eqP.
+  simpl. splitb; apply/eqP.
+  - apply no_source_c, vlabel_cv.
+  - move=> ?. contradict Hc. by apply ccl_eq.
+  - move=> ?. contradict Hc. apply one_target_c; trivial. apply vlabel_cv.
+  - move=> ?. contradict Hr. by apply right_eq2.
 Qed.
 
 Definition rem_node_transport' (e : edge rem_node_graph) : edge G :=
@@ -120,9 +116,9 @@ Definition rem_node_transport' (e : edge rem_node_graph) : edge G :=
 Lemma rem_node_transport'_inj : injective rem_node_transport'.
 Proof.
   assert (elv <> erv) by apply left_neq_right.
-  move => [[[[[e E] | []] | ]| []] | ] [[[[[a A] | []] | ]| []] | ];
+  move=> [[[[[e E] | []] | ]| []] | ] [[[[[a A] | []] | ]| []] | ];
   cbnb; introb; cbnb.
-  all: try by (contradict E || contradict A); apply /negP;
+  all: try by (contradict E || contradict A); apply/negP;
     rewrite rem_node_removed // !in_set !in_set1; caseb.
   by assert (erv <> elv) by by apply nesym.
 Qed.
@@ -130,23 +126,22 @@ Qed.
 Lemma rem_node_transportK e :
   e <> ecv -> rem_node_transport' (rem_node_transport e) = e.
 Proof.
-  intros ?.
-  unfold rem_node_transport, rem_node_transport'.
+  move=> ?.
+  rewrite /rem_node_transport /rem_node_transport'.
   case: {-}_ /boolP => In; cbnb. case_if.
-  revert In. rewrite rem_node_removed !in_set !in_set1. introb.
+  move: In. rewrite rem_node_removed !in_set !in_set1. introb.
 Qed.
 
-Lemma rem_node_transportK' e :
-  rem_node_transport (rem_node_transport' e) = e.
+Lemma rem_node_transportK' : cancel rem_node_transport' rem_node_transport.
 Proof.
-  unfold rem_node_transport, rem_node_transport'.
-  destruct e as [[[[[e E] | []] | ] | []] | ];
+  rewrite /rem_node_transport /rem_node_transport'.
+  move=> [[[[[e E] | []] | ] | []] | ];
   case: {-}_ /boolP => In.
   - cbnb.
-  - by contradict E; apply /negP.
-  - contradict In; apply /negP. rewrite rem_node_removed !in_set !in_set1. caseb.
+  - contradict E. by apply/negP.
+  - contradict In. apply/negP. by rewrite rem_node_removed !in_set !in_set1 eq_refl andb_false_r.
   - case_if. by assert (erv <> elv) by apply nesym, left_neq_right.
-  - contradict In; apply /negP. rewrite rem_node_removed !in_set !in_set1. caseb.
+  - contradict In. apply/negP. by rewrite rem_node_removed !in_set !in_set1 eq_refl !andb_false_r.
   - by rewrite eq_refl.
 Qed.
 
@@ -159,125 +154,125 @@ Lemma rem_node_transport_in_edges_at (b : bool) (e : edge G)
 Proof.
   rewrite in_set /rem_node_transport.
   case: {-}_ /boolP => In; cbnb; case_if; destruct b; cbnb.
-  - contradict Hu; apply /negP. rewrite !in_set !in_set1 left_e. caseb.
-  - revert In. rewrite rem_node_removed // !in_set !in_set1. introb.
-    all: contradict Hu; apply /negP; rewrite !in_set !in_set1 ?right_e; caseb.
-  - revert In. rewrite rem_node_removed // !in_set !in_set1. introb.
-    contradict Hu; apply /negP.
+  - contradict Hu; apply/negP. rewrite !in_set !in_set1 left_e. caseb.
+  - move: In. rewrite rem_node_removed // !in_set !in_set1. introb.
+    all: contradict Hu; apply/negP; rewrite !in_set !in_set1 ?right_e; caseb.
+  - move: In. rewrite rem_node_removed // !in_set !in_set1. introb.
+    contradict Hu; apply/negP.
     rewrite ccl_e !in_set !in_set1. caseb.
 Qed.
 
 Lemma rem_node_transport_edges u Hu b : edges_at_outin b u =
   [set rem_node_transport' a | a in edges_at_outin b (inl (inl (Sub u Hu)) : rem_node_graph)].
 Proof.
-  apply /setP => e. rewrite in_set.
+  apply/setP => e. rewrite in_set.
   symmetry. destruct (eq_comparable u (endpoint b e)) as [? | Hc]; [subst u | ].
-  - rewrite eq_refl. apply /imsetP. exists (rem_node_transport e).
+  - rewrite eq_refl. apply/imsetP. exists (rem_node_transport e).
     + apply rem_node_transport_in_edges_at.
     + rewrite rem_node_transportK //.
-      intros ?; subst e.
-      contradict Hu; apply /negP.
+      move=> ?; subst e.
+      contradict Hu; apply/negP.
       rewrite !in_set !in_set1.
       destruct b; rewrite ?ccl_e; caseb.
-  - transitivity false; last by by symmetry; apply /eqP; apply nesym.
-    apply /imsetP; move => [[[[[[a A] | []] | ] | []] | ] Ain /= ?]; subst e.
-    all: contradict Ain; apply /negP.
-    all: rewrite !in_set eq_sym; destruct b; cbnb; by apply /eqP.
+  - transitivity false; last by by symmetry; apply/eqP; apply nesym.
+    apply/imsetP; move=> [[[[[[a A] | []] | ] | []] | ] Ain /= ?]; subst e.
+    all: contradict Ain; apply/negP.
+    all: rewrite !in_set eq_sym; destruct b; cbnb; by apply/eqP.
 Qed.
 
 Lemma rem_node_p_deg : proper_degree rem_node_graph.
 Proof.
-  move => b [[[u U] | []] | []] /=.
+  move=> b [[[u U] | []] | []] /=.
   - rewrite -p_deg rem_node_transport_edges card_imset //; by apply rem_node_transport'_inj.
   - destruct b.
     + assert (Hr : edges_at_in (inl (inr tt) : rem_node_graph) = [set Some (inl None)]).
-      { apply /setP => e; rewrite !in_set in_set1. by destruct e as [[[[[? ?] | []] | ] | []] | ]. }
+      { apply/setP => e; rewrite !in_set in_set1. by destruct e as [[[[[? ?] | []] | ] | []] | ]. }
       by rewrite Hr cards1.
     + assert (Hr : edges_at_out (inl (inr tt) : rem_node_graph) = set0).
-      { apply /setP => e; rewrite !in_set. by destruct e as [[[[[? ?] | []] | ] | []] | ]. }
+      { apply/setP => e; rewrite !in_set. by destruct e as [[[[[? ?] | []] | ] | []] | ]. }
       by rewrite Hr cards0.
   - destruct b.
     + assert (Hr : edges_at_in (inr tt : rem_node_graph) = [set None]).
-      { apply /setP => e. rewrite !in_set in_set1. by destruct e as [[[[[? ?] | []] | ] | []] | ]. }
+      { apply/setP => e. rewrite !in_set in_set1. by destruct e as [[[[[? ?] | []] | ] | []] | ]. }
       by rewrite Hr cards1.
     + assert (Hr : edges_at_out (inr tt : rem_node_graph) = set0).
-      { apply /setP => e. rewrite !in_set. by destruct e as [[[[[? ?] | []] | ] | []] | ]. }
+      { apply/setP => e. rewrite !in_set. by destruct e as [[[[[? ?] | []] | ] | []] | ]. }
       by rewrite Hr cards0.
 Qed.
 
 Lemma rem_node_p_ax_cut : proper_ax_cut rem_node_graph.
 Proof.
-  move => b [[[u U] | []] | []] /= Hu; try by destruct b.
+  move=> b [[[u U] | []] | []] /= Hu; try by destruct b.
   destruct (p_ax_cut Hu) as [el [er [Lin [Rin LR]]]].
   exists (rem_node_transport el), (rem_node_transport er).
-  revert Lin. rewrite rem_node_transport_edges => /imsetP[al Al ?]. subst el.
-  revert Rin. rewrite rem_node_transport_edges => /imsetP[ar Ar ?]. subst er.
-  revert LR. rewrite !flabel_rem_node_transport' => LR.
+  move: Lin. rewrite rem_node_transport_edges => /imsetP[al Al ?]. subst el.
+  move: Rin. rewrite rem_node_transport_edges => /imsetP[ar Ar ?]. subst er.
+  move: LR. rewrite !flabel_rem_node_transport' => LR.
   rewrite !rem_node_transportK'. splitb.
 Qed.
 
 Lemma rem_node_p_tens_parr : proper_tens_parr rem_node_graph.
 Proof.
-  move => b [[[u U] | []] | []] /= Hu; try by destruct b.
+  move=> b [[[u U] | []] | []] /= Hu; try by destruct b.
   destruct (p_tens_parr Hu) as [el [er [ec [Lin [Ll [Rin [Rl [Cin Elrc]]]]]]]].
   exists (rem_node_transport el), (rem_node_transport er), (rem_node_transport ec).
-  revert Lin. rewrite rem_node_transport_edges => /imsetP[al Al ?]. subst el.
-  revert Rin. rewrite rem_node_transport_edges => /imsetP[ar Ar ?]. subst er.
-  revert Cin. rewrite rem_node_transport_edges => /imsetP[ac Ac ?]. subst ec.
-  revert Elrc. rewrite !flabel_rem_node_transport' => Elrc.
+  move: Lin. rewrite rem_node_transport_edges => /imsetP[al Al ?]. subst el.
+  move: Rin. rewrite rem_node_transport_edges => /imsetP[ar Ar ?]. subst er.
+  move: Cin. rewrite rem_node_transport_edges => /imsetP[ac Ac ?]. subst ec.
+  move: Elrc. rewrite !flabel_rem_node_transport' => Elrc.
   rewrite !rem_node_transportK'. splitb.
-  - revert Ll. destruct al as [[[[[? ?] | []] | ] | []] | ]; cbnb.
-  - revert Rl. destruct ar as [[[[[? ?] | []] | ] | []] | ]; cbnb.
+  - move: Ll. destruct al as [[[[[? ?] | []] | ] | []] | ]; cbnb.
+  - move: Rl. destruct ar as [[[[[? ?] | []] | ] | []] | ]; cbnb.
     + contradict Ar. by rewrite !in_set.
     + by rewrite left_l.
 Qed.
 
 Lemma rem_node_p_noleft : proper_noleft rem_node_graph.
-Proof. move => [[[[[e E] | []] | ]| []] | ] //=. by apply p_noleft. Qed.
+Proof. move=> [[[[[e E] | []] | ]| []] | ] //=. by apply p_noleft. Qed.
 
 Lemma rem_node_p_order_full : proper_order_full rem_node_graph_data.
 Proof.
   rewrite /= /rem_node_order.
-  move => [[[[[e E] | []] | ] | []] | ] //=.
+  move=> [[[[[e E] | []] | ] | []] | ] //=.
   rewrite !in_cons /=.
   assert (Hr : Some (inl (Some (inl (Sub e E : edge rem_node_graph_1)))) = rem_node_transport e).
   { rewrite /rem_node_transport. case: {-}_ /boolP => [In | /negP //]. cbnb. }
   rewrite Hr {Hr}. split.
-  - move => ?. apply map_f.
+  - move=> ?. apply map_f.
     rewrite mem_filter. splitb.
-    + revert E. rewrite rem_node_removed !in_set !in_set1. introb.
+    + move: E. rewrite rem_node_removed !in_set !in_set1. introb.
     + by apply p_order_full.
-  - move => /mapP[a A Ha].
+  - move=> /mapP[a A Ha].
     assert (a = e).
-    { revert Ha. unfold rem_node_transport. case: {-}_ /boolP => [In | /negP //].
+    { move: Ha. unfold rem_node_transport. case: {-}_ /boolP => [In | /negP //].
       case: {-}_ /boolP => [In' | /negP-? //]; last by case_if.
-      move => /eqP. by cbnb => /eqP-->. }
+      move=> /eqP. by cbnb => /eqP-->. }
     subst a.
-    revert A. rewrite mem_filter. introb.
+    move: A. rewrite mem_filter. introb.
     by apply p_order_full.
 Qed.
 
 Lemma rem_node_p_order_uniq : proper_order_uniq rem_node_graph_data.
 Proof.
   rewrite /proper_order_uniq /= in_cons /=. splitb.
-  - apply /mapP; move => [a A] /eqP.
+  - apply/mapP; move=> [a A] /eqP.
     rewrite /rem_node_transport.
     case: {-}_ /boolP => ?; case_if.
-    revert A. rewrite mem_filter => /andP[_ A].
+    move: A. rewrite mem_filter => /andP[_ A].
     apply p_order_full in A.
     contradict A.
     rewrite left_e. by destruct V as [H | H]; rewrite H.
-  - apply /mapP; move => [a A] /eqP.
+  - apply/mapP; move=> [a A] /eqP.
     rewrite /rem_node_transport.
     case: {-}_ /boolP => Ain; case_if.
-    revert A. rewrite mem_filter => /andP[/eqP-A0 A].
-    revert Ain. rewrite rem_node_removed // !in_set !in_set1. introb.
+    move: A. rewrite mem_filter => /andP[/eqP-A0 A].
+    move: Ain. rewrite rem_node_removed // !in_set !in_set1. introb.
     apply p_order_full in A.
     contradict A.
     rewrite right_e. by destruct V as [H | H]; rewrite H.
   - rewrite map_inj_in_uniq.
     { apply filter_uniq, p_order_uniq. }
-    intros a b.
+    move=> a b.
     rewrite !mem_filter => /andP[_ A] /andP[_ B].
     rewrite /rem_node_transport.
     case: {-}_ /boolP => Ain;
@@ -285,9 +280,9 @@ Proof.
     enough (L : forall e, e \notin edge_set (setT :\ v :\ cv) -> e \in order G -> e = ecv).
     { transitivity (ccl V); [ | symmetry]; by apply L. }
     clear - T.
-    intros a Ain A.
+    move=> a Ain A.
     apply p_order_full in A.
-    revert Ain. rewrite rem_node_removed !in_set !in_set1. introb.
+    move: Ain. rewrite rem_node_removed !in_set !in_set1. introb.
     + contradict A. rewrite right_e. destruct V as [H | H]; by rewrite H.
     + contradict A. rewrite left_e. destruct V as [H | H]; by rewrite H.
 Qed.
@@ -306,8 +301,7 @@ End Rem_node.
 
 
 Section Sequentializing_parr.
-Context {G : proof_net} {v : G}.
-Hypothesis (V : vlabel v = ⅋) (T : terminal v).
+Context {G : proof_net} {v : G} (V : vlabel v = ⅋) (T : terminal v).
 
 (* Vertices neighbourhing v *)
 Local Notation elv := (left_parr V).
@@ -396,7 +390,7 @@ Proof.
   rewrite /rem_parr_v_bij_fwd /rem_parr_v_bij_bwd SubK /rem_parr_v_bij_bwd_1.
   case: {-}_ /boolP => [// | Ul].
   case: ifP => [/eqP--> // | /eqP/eqP-UV] /=.
-  symmetry. apply /eqP. by apply rem_parr_v_bij_bwd_last_case.
+  symmetry. apply/eqP. by apply rem_parr_v_bij_bwd_last_case.
 Qed.
 
 Definition rem_parr_iso_v := {|
